
# Binomial

$Binomial = Monomial + Monomial$ <br>
$= x_{0}^{x_{0}} * \cdots + x_{0}^{x_{0}} * \cdots$ <br>
$x \neq 0$ <br>
$n \geq 0$ <br>

<br>
<br>

## Examples

- $x + y = x^{1} + y^{1}$

- $3x^{2} - xy^{4} = 3^{1} * x^{2} + (-1)^{1} * x^{1} * y^{4}$

<br>
<br>

## Expansions

-   $a^{n} - b^{n} = (a - b) * \sum{x = 0}^{n - 1} a^{k} * b^{n - 1 - k}$

    $a^{2} - b^{2} = (a - b)(a^{0} * b^{1} + a^{1} * b^{0})$
    $= (a - b)(a + b)$
    
    $a^{3} - b^{3} = (a - b)(a^{0} * b^{2} + a^{1} * b^{1} + a^{2} * b^{0})$
    $= (a - b)(a^{2} + ab + b^{2})$
    
-   $(a + b)(c + d) = ac + ad + bc + bd$

-   $a^{3} \pm b^{3} = (a \pm b)(a^{2} \mp ab + b^{2})$

-   **[Binomial Theorem]**

<br>


<!----------------------------------------------------------------------------->

[Binomial Theorem]: ../Misc/Binomial%20Theorem.md
