
# Trigonometric Integrals

<br>
<br>

$\displaystyle\huge sin  x  \overset{\normalsize{\int}}{⟶}  - cos  x + C$
  
<br>
<br>
  
$\displaystyle\huge cos  x  \overset{\normalsize{\int}}{⟶}  + sin  x + C$
  
<br>
<br>
  
$\displaystyle\huge tan  x  \overset{\normalsize{\int}}{⟶}  + \ln{| \sec  x  |} + C$ <br>
$\displaystyle\huge             =    - \ln{| \cos  x |} + C$
  
<br>
<br>
  
$\displaystyle\huge cot  x  \overset{\normalsize{\int}}{⟶}  \ln{| \sin  x  |} + C$ <br>

<br>
<br>

$\displaystyle\huge sec  x  \overset{\normalsize{\int}}{⟶}  + \ln{| \sec  x + \tan  x  |} + C$ <br>
$\displaystyle\huge             =    - \ln{|  \tan (  \frac{x}{2} + \frac{\pi}{4} )  |} + C$

<br>
<br>

$\displaystyle\huge csc  x  \overset{\normalsize{\int}}{⟶}  - \ln{| \csc  x + \cot  x  |} + C$ <br>
$\displaystyle\huge             =     + \ln{| \csc  x - \cot  x  |} + C$ <br>
$\displaystyle\huge             =     + \ln{|             \tan \frac{x}{2}              |} + C$
  
<br>
<br>

## Inverses

<br>
<br>

$\displaystyle\huge\overline{\overset{\vphantom{\\\_}}{sin}}  x  \overset{\normalsize{\int}}{⟶}  x \ast \overline{\overset{\vphantom{\\\_}}{sin}}  x + \underset{\underset{                       \leq 0}{\vphantom{.}}}{\sqrt{1 - x^{ 2}}} + C$

<br>
<br>
  
$\displaystyle\huge\overline{\overset{\vphantom{\\\_}}{cos}}  x  \overset{\normalsize{\int}}{⟶}  x \ast \overline{\overset{\vphantom{\\\_}}{cos}}  x - \underset{\underset{                       \leq 0}{\vphantom{.}}}{\sqrt{1 - x^{ 2}}} + C$

<br>
<br>
  
$\displaystyle\huge\overline{\overset{\vphantom{\\\_}}{tan}}  x  \overset{\normalsize{\int}}{⟶}  x \ast \overline{\overset{\vphantom{\\\_}}{tan}}  x - \frac{1}{2} * \ln{| 1 + x^{ 2} |} + C$
  
<br>
<br>
  
$\displaystyle\huge\overline{\overset{\vphantom{\\\_}}{cot}}  x  \overset{\normalsize{\int}}{⟶}  x \ast \overline{\overset{\vphantom{\\\_}}{cot}}  x + \frac{1}{2} * \ln{| 1 + x^{ 2} |} + C$
  
<br>
<br>
  
$\displaystyle\huge\overline{\overset{\vphantom{\\\_}}{sec}}  x  \overset{\normalsize{\int}}{⟶}  x \ast \overline{\overset{\vphantom{\\\_}}{sec}}  x - \ln{| x * ( 1 + \underset{\underset{                 \geq 0}{\vphantom{.}}}{\sqrt{ 1 - x^{ - 2} }} ) |} + C$

<br>
<br>
  
$\displaystyle\huge\overline{\overset{\vphantom{\\\_}}{csc}}  x  \overset{\normalsize{\int}}{⟶}  x \ast \overline{\overset{\vphantom{\\\_}}{csc}}  x + \ln{| x * ( 1 + \underset{\underset{                 \geq 0}{\vphantom{.}}}{\sqrt{ 1 - x^{ - 2} }} ) |} + C$

<br>
