
# Binomial Theorem

<br>

$\large (a + b)^{n} = \displaystyle\sum_{k = 0}^{n} \left( \begin{array}{c} n \\\\ k \end{array} \right) a^{k} * b^{n - k}$

$\large                       = \displaystyle\sum_{k = 0}^{n} \left( \begin{array}{c} n \\\\ k \end{array} \right) a^{n - k} * b^{k}$

<br>
<br>

## Examples

<br>

-   $\large (a + b)^{0} =                          1$

    <br>

-   $\large (a + b)^{1} = a                     +                     b$

    <br>

-   $\large (a + b)^{2} = a^{2} +            2ab            + b^{2}$

    <br>

-   $\large (a + b)^{3} = a^{3} + 3a^{2}b + 3ab^{2} + b^{3}$

<br>
